Merged and added some changes to memory

src/Dafny/memory.dfy
@@ -4,12 +4,9 @@ module memory {
 
 import opened types
 
-// TEMPORARY
-datatype ptr = ptr(bid:nat, offset:nat)
-
 // Each cell of memory is occupied by either data, a pointer, or uninitialized
 // data
-datatype MemCell =  mb(size:nat, data:byte) | 
+datatype MemCell =  mb(size:nat, data:uint8) | 
                     mptr(block:nat, offset:nat, index:nat) |
                     muninit()
 
@@ -37,13 +34,12 @@ function UninitBlock(size:nat) : (b:Block)
 
 // Pointers and block indices can be valid/invalid depending on whether the
 // location exists in memory
-predicate IsValidBlock(s:MemState, bid:nat) {
-    bid in s.mem
+predicate IsValidBid(s:MemState, bid:nat) {
+	bid in s.mem
 }
-
-predicate IsValidPtr(s:MemState, p:ptr) {
-    && p.bid in s.mem
-    && p.offset < |s.mem[p.bid]|
+predicate IsValidPtr(s:MemState, bid:nat, offset:nat) {
+	&& bid in s.mem
+	&& offset < |s.mem[bid]|
 }
 
 // On initialization, the memory state is empty and contains no blocks
@@ -52,9 +48,28 @@ predicate MemInit(s:MemState) {
     && s.nextBlock == 0
 }
 
+// A byte-memory cell is valid within a block if the surrounding memory cells starting
+// at the appropriate alignment are of the same size
+predicate ByteMemValid(b:Block, offset:nat)
+	requires offset < |b|
+	requires b[offset].mb?
+	requires b[offset].size > 0
+{
+	var cell := b[offset];
+	var align:nat := offset - (offset % cell.size);
+	forall i | align <= i < (align + cell.size) :: (i < |b| && b[i].mb? && b[i].size == cell.size)
+}
+
+// A block is valid so long as its stored bytes are well-formed; that is, numbers
+// of size n start on an index divisible by n and fill the entire n space
+predicate BlockValid(b:Block) {
+	forall offset | 0 <= offset < |b| :: (b[offset].mb? ==> (b[offset].size > 0 && ByteMemValid(b, offset)))
+}
+
 // Need to check every step to make sure memory is still valid
 predicate MemValid(s:MemState) {
-    forall bid | bid in s.mem :: bid < s.nextBlock
+	&& (forall bid | bid in s.mem :: bid < s.nextBlock)
+	&& (forall bid | bid in s.mem :: BlockValid(s.mem[bid]))
 }
 
 // When a new block is allocated, all the previous blocks should remain the same,
@@ -67,30 +82,32 @@ predicate Alloc(s:MemState, s':MemState, bid:nat, size:nat) {
 }
 
 // Blocks can be freed as well, in which case it is simply removed from the map
-predicate Free(s:MemState, s':MemState, bid:nat)
-    requires IsValidBlock(s, bid)
-{
-    && s'.nextBlock == s.nextBlock
-    && bid !in s'.mem
-    && s.mem == s'.mem[bid:= s.mem[bid]]
+predicate Free(s:MemState, s':MemState, bid:nat) {
+	&& s'.nextBlock == s.nextBlock
+	&& IsValidBid(s, bid)
+	&&! IsValidBid(s', bid)
+	&& s.mem == s'.mem[bid:= s.mem[bid]]
 }
 
 // TODO: Support reading and writing more than one byte at a time
-predicate Load(s:MemState, s':MemState, p:ptr, val:byte)
-    requires IsValidPtr(s, p)
-{
-    var cell := s.mem[p.bid][p.offset];
-    && s' == s
-    && cell.mb?
-    && cell.data == val
+predicate Load(s:MemState, s':MemState, bid:nat, offset:nat, data:Data) {
+	if !IsValidPtr(s, bid, offset) || data.Ptr? then false
+	else
+		var bytes := (if data.Bytes? then data.bytes else IntToBytes(data));
+		&& (s' == s)
+		&& (data.Int? ==> offset % |bytes| == 0)
+		&& (offset + |bytes| <= |s.mem[bid]|)
+		&& (forall i | 0 <= i < |bytes| :: (offset + i < |s.mem[bid]|))
+		&& (forall i | 0 <= i < |bytes| :: s.mem[bid][offset + i].mb?)
 }
 
 // TODO: Support reading and writing more than one byte at a time
-predicate Store(s:MemState, s':MemState, p:ptr, val:byte)
-    requires IsValidPtr(s, p)
+predicate Store(s:MemState, s':MemState, bid:nat, offset:nat, data:Data)
+	requires IsValidPtr(s, bid, offset)
 {
-    && s'.nextBlock == s.nextBlock
-    && s'.mem == s.mem[p.bid := s.mem[p.bid][p.offset := mb(1, val)]]
+	true
+	// && s'.nextBlock == s.nextBlock
+	// && s'.mem == s.mem[p.bid := s.mem[p.bid][p.offset := mb(1, val)]]
 }
 
 
